fstar/new/MLS.NetworkBinder.fst
@@ -24,20 +24,20 @@ let option_to_network #a opt =
 
 
 noeq type leaf_package_content_nt = {
-  lpc_public_key: hpke_public_key_nt;
+  public_key: hpke_public_key_nt;
 }
 
 val ps_leaf_package_content: parser_serializer leaf_package_content_nt
 let ps_leaf_package_content =
   isomorphism leaf_package_content_nt
     ps_hpke_public_key
-    (fun public_key -> ({lpc_public_key = public_key}))
-    (fun x -> x.lpc_public_key)
+    (fun public_key -> ({public_key = public_key}))
+    (fun x -> x.public_key)
 
 noeq type node_package_content_nt = {
-  npc_public_key: hpke_public_key_nt;
-  npc_encrypted_path_secret: blseq hpke_ciphertext_nt ps_hpke_ciphertext ({min=0; max=(pow2 32)-1});
-  npc_last_group_context: blbytes ({min=0; max=(pow2 64) - 1});
+  public_key: hpke_public_key_nt;
+  encrypted_path_secret: blseq hpke_ciphertext_nt ps_hpke_ciphertext ({min=0; max=(pow2 32)-1});
+  last_group_context: blbytes ({min=0; max=(pow2 64) - 1});
 }
 
 val ps_node_package_content: parser_serializer node_package_content_nt
@@ -49,117 +49,117 @@ let ps_node_package_content =
       _ <-- ps_seq _ ps_hpke_ciphertext;
       ps_bytes _
     )
-    (fun (|public_key, (|encrypted_path_secret, last_group_context|)|) -> ({npc_public_key = public_key; npc_encrypted_path_secret = encrypted_path_secret; npc_last_group_context = last_group_context;}))
-    (fun x -> (|x.npc_public_key, (|x.npc_encrypted_path_secret, x.npc_last_group_context|)|))
+    (fun (|public_key, (|encrypted_path_secret, last_group_context|)|) -> ({public_key = public_key; encrypted_path_secret = encrypted_path_secret; last_group_context = last_group_context;}))
+    (fun x -> (|x.public_key, (|x.encrypted_path_secret, x.last_group_context|)|))
 
 
 (*** NetworkTreeSyncBinder ***)
 
 val key_package_to_treesync: key_package_nt -> result TS.leaf_package_t
 let key_package_to_treesync kp =
-  match kp.kpn_credential with
+  match kp.credential with
   | C_basic cred ->
     return ({
-      TS.lp_credential = {
-        TS.cred_version = 0;
-        TS.cred_identity = cred.bcn_identity;
-        TS.cred_signature_key = cred.bcn_signature_key;
+      TS.credential = {
+        TS.version = 0;
+        TS.identity = cred.identity;
+        TS.signature_key = cred.signature_key;
       };
-      TS.lp_version = 0;
-      TS.lp_content = ps_leaf_package_content.serialize ({lpc_public_key = kp.kpn_public_key});
-      TS.lp_extensions = (ps_seq _ ps_extension).serialize (kp.kpn_extensions);
-      TS.lp_signature = kp.kpn_signature;
+      TS.version = 0;
+      TS.content = ps_leaf_package_content.serialize ({public_key = kp.public_key});
+      TS.extensions = (ps_seq _ ps_extension).serialize (kp.extensions);
+      TS.signature = kp.signature;
     })
   | _ -> error "key_package_to_treesync: credential type not supported"
 
 val treesync_to_keypackage: ciphersuite -> TS.leaf_package_t -> result key_package_nt
 let treesync_to_keypackage cs lp =
-  if not (Seq.length lp.TS.lp_credential.TS.cred_identity < pow2 16) then
-    error "treesync_to_keypackage: cred_identity too long"
-  else if not (Seq.length lp.TS.lp_credential.TS.cred_signature_key < pow2 16) then
-    error "treesync_to_keypackage: cred_signature_key too long"
-  else if not (Seq.length lp.TS.lp_signature < pow2 16) then
+  if not (Seq.length lp.TS.credential.TS.identity < pow2 16) then
+    error "treesync_to_keypackage: identity too long"
+  else if not (Seq.length lp.TS.credential.TS.signature_key < pow2 16) then
+    error "treesync_to_keypackage: signature_key too long"
+  else if not (Seq.length lp.TS.signature < pow2 16) then
     error "treesync_to_keypackage: signature too long"
   else (
-    leaf_content <-- from_option "treesync_to_keypackage: can't parse leaf content" ((ps_to_pse ps_leaf_package_content).parse_exact lp.TS.lp_content);
-    extensions <-- from_option "treesync_to_keypackage: can't parse extensions" ((ps_to_pse (ps_seq _ ps_extension)).parse_exact lp.TS.lp_extensions);
+    leaf_content <-- from_option "treesync_to_keypackage: can't parse leaf content" ((ps_to_pse ps_leaf_package_content).parse_exact lp.TS.content);
+    extensions <-- from_option "treesync_to_keypackage: can't parse extensions" ((ps_to_pse (ps_seq _ ps_extension)).parse_exact lp.TS.extensions);
     cipher_suite <-- ciphersuite_to_nt cs;
     return ({
-      kpn_version = PV_mls10;
-      kpn_cipher_suite = cipher_suite;
-      kpn_public_key = leaf_content.lpc_public_key;
-      kpn_credential = C_basic ({
-        bcn_identity = lp.TS.lp_credential.TS.cred_identity;
-        bcn_signature_scheme = SA_ed25519; //TODO
-        bcn_signature_key = lp.TS.lp_credential.TS.cred_signature_key;
+      version = PV_mls10;
+      cipher_suite = cipher_suite;
+      public_key = leaf_content.public_key;
+      credential = C_basic ({
+        identity = lp.TS.credential.TS.identity;
+        signature_scheme = SA_ed25519; //TODO
+        signature_key = lp.TS.credential.TS.signature_key;
       });
-      kpn_extensions = extensions;
-      kpn_signature = lp.TS.lp_signature;
-    })
+      extensions = extensions;
+      signature = lp.TS.signature;
+    } <: key_package_nt)
   )
 
 val treesync_to_parent_node: TS.node_package_t -> result parent_node_nt
 let treesync_to_parent_node np =
-  unmerged_leaves <-- mapM (fun (x:nat) -> if x < pow2 32 then return (Lib.IntTypes.u32 x) else internal_failure "") np.TS.np_unmerged_leafs;
-  if not (Seq.length np.TS.np_parent_hash < 256) then
+  unmerged_leaves <-- mapM (fun (x:nat) -> if x < pow2 32 then return (Lib.IntTypes.u32 x) else internal_failure "") np.TS.unmerged_leafs;
+  if not (Seq.length np.TS.parent_hash < 256) then
     internal_failure "treesync_to_parent_node: parent_hash too long"
   else if not ((byte_length ps_u32 unmerged_leaves) < pow2 32) then
     internal_failure "treesync_to_parent_node: unmerged_leaves too long"
   else (
     Seq.lemma_list_seq_bij unmerged_leaves;
-    node_content <-- from_option "treesync_to_parent_node: can't parse np_content" ((ps_to_pse ps_node_package_content).parse_exact np.TS.np_content);
+    node_content <-- from_option "treesync_to_parent_node: can't parse content" ((ps_to_pse ps_node_package_content).parse_exact np.TS.content);
     return ({
-      pnn_public_key = node_content.npc_public_key;
-      pnn_parent_hash = np.TS.np_parent_hash;
-      pnn_unmerged_leaves = Seq.seq_of_list unmerged_leaves;
-    })
+      public_key = node_content.public_key;
+      parent_hash = np.TS.parent_hash;
+      unmerged_leaves = Seq.seq_of_list unmerged_leaves;
+    } <: parent_node_nt)
   )
 
 val parent_node_to_treesync: parent_node_nt -> result TS.node_package_t
 let parent_node_to_treesync pn =
   return ({
-        TS.np_version = 0;
-        TS.np_content_dir = Left; //We don't care I guess
-        TS.np_unmerged_leafs = List.Tot.map (fun x -> let open Lib.IntTypes in (v x <: nat)) (Seq.seq_to_list pn.pnn_unmerged_leaves);
-        TS.np_parent_hash = pn.pnn_parent_hash;
-        TS.np_content = ps_node_package_content.serialize ({
-          npc_public_key = pn.pnn_public_key;
-          npc_encrypted_path_secret = Seq.empty;
-          npc_last_group_context = bytes_empty;
+        TS.version = 0;
+        TS.content_dir = Left; //We don't care I guess
+        TS.unmerged_leafs = List.Tot.map (fun x -> let open Lib.IntTypes in (v x <: nat)) (Seq.seq_to_list pn.unmerged_leaves);
+        TS.parent_hash = pn.parent_hash;
+        TS.content = ps_node_package_content.serialize ({
+          public_key = pn.public_key;
+          encrypted_path_secret = Seq.empty;
+          last_group_context = bytes_empty;
         });
-      })
+      } <: TS.node_package_t)
 
 val key_package_to_treekem: cs:ciphersuite -> key_package_nt -> result (TK.member_info cs)
 let key_package_to_treekem cs kp =
-  if not (Seq.length kp.kpn_public_key = hpke_public_key_length cs) then
+  if not (Seq.length kp.public_key = hpke_public_key_length cs) then
     error "key_package_to_treekem: public key has wrong length"
   else
     return ({
-      TK.mi_public_key = kp.kpn_public_key;
-      TK.mi_version = 0;
-    })
+      TK.public_key = kp.public_key;
+      TK.version = 0;
+    } <: TK.member_info cs)
 
 val update_path_node_to_treekem: cs:ciphersuite -> bytes -> direction -> update_path_node_nt -> result (TK.key_package cs)
 let update_path_node_to_treekem cs group_context dir update_path_node =
-  if not (Seq.length update_path_node.upnn_public_key = hpke_public_key_length cs) then
+  if not (Seq.length update_path_node.public_key = hpke_public_key_length cs) then
     error "update_path_node_to_treekem: public key has wrong length"
   else (
-    path_secret_ciphertext <-- mapM (fun hpke_ciphertext ->
-      if not (Seq.length hpke_ciphertext.hcn_kem_output = hpke_kem_output_length cs) then
+    path_secret_ciphertext <-- mapM (fun (hpke_ciphertext: hpke_ciphertext_nt) ->
+      if not (Seq.length hpke_ciphertext.kem_output = hpke_kem_output_length cs) then
         error "update_path_node_to_treekem: kem output has wrong length"
       else
         return ({
-          TK.kem_output = hpke_ciphertext.hcn_kem_output;
-          TK.ciphertext = hpke_ciphertext.hcn_ciphertext;
+          TK.kem_output = hpke_ciphertext.kem_output;
+          TK.ciphertext = hpke_ciphertext.ciphertext;
         })
-    ) (Seq.seq_to_list update_path_node.upnn_encrypted_path_secret);
+    ) (Seq.seq_to_list update_path_node.encrypted_path_secret);
     return ({
-      TK.kp_public_key = update_path_node.upnn_public_key;
-      TK.kp_version = 0;
-      TK.kp_last_group_context = group_context;
-      TK.kp_unmerged_leafs = [];
-      TK.kp_path_secret_from = dir;
-      TK.kp_path_secret_ciphertext = path_secret_ciphertext;
+      TK.public_key = update_path_node.public_key;
+      TK.version = 0;
+      TK.last_group_context = group_context;
+      TK.unmerged_leafs = [];
+      TK.path_secret_from = dir;
+      TK.path_secret_ciphertext = path_secret_ciphertext;
     })
   )
 
@@ -167,25 +167,25 @@ let update_path_node_to_treekem cs group_context dir update_path_node =
 val update_path_to_treekem: cs:ciphersuite -> l:nat -> n:tree_size l -> i:leaf_index n -> bytes -> update_path:update_path_nt -> result (TK.pathkem cs l n i)
 let rec update_path_to_treekem cs l n i group_context update_path =
   if l = 0 then (
-    if not (Seq.length update_path.upn_nodes = 0) then
+    if not (Seq.length update_path.nodes = 0) then
       internal_failure "update_path_to_treekem: update_path.nodes is too long"
     else (
-      leaf_package <-- key_package_to_treekem cs update_path.upn_leaf_key_package;
+      leaf_package <-- key_package_to_treekem cs update_path.leaf_key_package;
       return (PLeaf leaf_package)
     )
   ) else if (n <= pow2 (l-1)) then (
     path_next <-- update_path_to_treekem cs (l-1) n i group_context update_path;
     return (PSkip _ path_next)
   ) else (
-    if not (Seq.length update_path.upn_nodes > 0) then
+    if not (Seq.length update_path.nodes > 0) then
       internal_failure "update_path_to_treekem: update_path.nodes is too short"
     else (
-      let update_path_length = (Seq.length update_path.upn_nodes) in
-      let head_update_path_nodes = Seq.index update_path.upn_nodes (update_path_length-1) in
-      let tail_update_path_nodes = Seq.slice update_path.upn_nodes 0 (update_path_length-1) in
+      let update_path_length = (Seq.length update_path.nodes) in
+      let head_update_path_nodes = Seq.index update_path.nodes (update_path_length-1) in
+      let tail_update_path_nodes = Seq.slice update_path.nodes 0 (update_path_length-1) in
       //TODO this is an easy lemma
-      assume (byte_length ps_update_path_node (Seq.seq_to_list tail_update_path_nodes) <= byte_length ps_update_path_node (Seq.seq_to_list update_path.upn_nodes));
-      let next_update_path = { update_path with upn_nodes = tail_update_path_nodes } in
+      assume (byte_length ps_update_path_node (Seq.seq_to_list tail_update_path_nodes) <= byte_length ps_update_path_node (Seq.seq_to_list update_path.nodes));
+      let next_update_path = { update_path with nodes = tail_update_path_nodes } in
       let (|dir, next_i|) = child_index l i in
       path_next <-- update_path_to_treekem cs (l-1) (if dir = Left then pow2 (l-1) else n - (pow2 (l-1))) next_i group_context next_update_path;
       path_data <-- update_path_node_to_treekem cs group_context dir head_update_path_nodes;
@@ -198,9 +198,9 @@ let rec update_path_to_treekem cs l n i group_context update_path =
 
 val dumb_credential: TS.credential_t
 let dumb_credential = {
-  TS.cred_version = 0;
-  TS.cred_identity = Seq.empty;
-  TS.cred_signature_key = Seq.empty;
+  TS.version = 0;
+  TS.identity = Seq.empty;
+  TS.signature_key = Seq.empty;
 }
 
 val ratchet_tree_l_n: nodes:ratchet_tree_nt -> result (l:nat & n:tree_size l{Seq.length nodes == n+n-1})
