fstar/new/MLS.TreeDEM.Message.Framing.fst
@@ -18,71 +18,71 @@ type sender_type =
   | ST_new_member
 
 type sender = {
-  s_sender_type: sender_type;
-  s_sender_id: nat;
+  sender_type: sender_type;
+  sender_id: nat;
 }
 
 noeq type message = {
-  m_group_id: bytes;
-  m_epoch: nat;
-  m_sender: sender;
-  m_authenticated_data: bytes;
-  m_content_type: message_content_type;
-  m_message_content: message_content m_content_type;
+  group_id: bytes;
+  epoch: nat;
+  sender: sender;
+  authenticated_data: bytes;
+  content_type: message_content_type;
+  message_content: message_content content_type;
 }
 
 noeq type message_auth = {
-  m_signature: bytes;
-  m_confirmation_tag: option bytes;
+  signature: bytes;
+  confirmation_tag: option bytes;
 }
 
 noeq type message_plaintext = {
-  mp_group_id: bytes;
-  mp_epoch: nat;
-  mp_sender: sender;
-  mp_authenticated_data: bytes;
-  mp_content_type: message_content_type;
-  mp_message_content: message_content mp_content_type;
-  mp_signature: bytes;
-  mp_confirmation_tag: option bytes;
-  mp_membership_tag: option bytes;
+  group_id: bytes;
+  epoch: nat;
+  sender: sender;
+  authenticated_data: bytes;
+  content_type: message_content_type;
+  message_content: message_content content_type;
+  signature: bytes;
+  confirmation_tag: option bytes;
+  membership_tag: option bytes;
 }
 
 noeq type message_ciphertext = {
-  mc_group_id: bytes;
-  mc_epoch: nat;
-  mc_content_type: message_content_type;
-  mc_authenticated_data: bytes;
-  mc_encrypted_sender_data: bytes;
-  mc_ciphertext: bytes;
+  group_id: bytes;
+  epoch: nat;
+  content_type: message_content_type;
+  authenticated_data: bytes;
+  encrypted_sender_data: bytes;
+  ciphertext: bytes;
 }
 
 noeq type message_ciphertext_content (content_type:message_content_type) = {
-  mcc_message_content: message_content content_type;
-  mcc_signature: bytes;
-  mcc_confirmation_tag: option bytes;
-  mcc_padding: bytes;
+  message_content: message_content content_type;
+  signature: bytes;
+  confirmation_tag: option bytes;
+  padding: bytes;
 }
 
 noeq type encrypted_sender_data_content = {
-  esdc_sender: nat;
-  esdc_generation: nat;
-  esdc_reuse_guard: lbytes 4;
+  sender: nat;
+  generation: nat;
+  reuse_guard: lbytes 4;
 }
 
 val message_plaintext_to_message: message_plaintext -> message & message_auth
 let message_plaintext_to_message pt =
-  ({
-    m_group_id = pt.mp_group_id;
-    m_epoch = pt.mp_epoch;
-    m_sender = pt.mp_sender;
-    m_authenticated_data = pt.mp_authenticated_data;
-    m_content_type = pt.mp_content_type;
-    m_message_content = pt.mp_message_content;
-  }, {
-    m_signature = pt.mp_signature;
-    m_confirmation_tag = pt.mp_confirmation_tag;
-  })
+  (({
+    group_id = pt.group_id;
+    epoch = pt.epoch;
+    sender = pt.sender;
+    authenticated_data = pt.authenticated_data;
+    content_type = pt.content_type;
+    message_content = pt.message_content;
+  } <: message), ({
+    signature = pt.signature;
+    confirmation_tag = pt.confirmation_tag;
+  } <: message_auth))
 
 val network_to_sender_type: sender_type_nt -> result sender_type
 let network_to_sender_type s =
@@ -101,21 +101,21 @@ let sender_type_to_network s =
 
 val network_to_sender: sender_nt -> result sender
 let network_to_sender s =
-  sender_type <-- network_to_sender_type s.sn_sender_type;
+  sender_type <-- network_to_sender_type s.sender_type;
   return ({
-    s_sender_type = sender_type;
-    s_sender_id = Lib.IntTypes.v s.sn_sender;
+    sender_type = sender_type;
+    sender_id = Lib.IntTypes.v s.sender;
   })
 
 val sender_to_network: sender -> result sender_nt
 let sender_to_network s =
-  if not (s.s_sender_id < pow2 32) then (
+  if not (s.sender_id < pow2 32) then (
     internal_failure "network_to_sender: sender_id too big"
   ) else (
     return ({
-      sn_sender_type = sender_type_to_network s.s_sender_type;
-      sn_sender = u32 s.s_sender_id;
-    })
+      sender_type = sender_type_to_network s.sender_type;
+      sender = u32 s.sender_id;
+    } <: sender_nt)
   )
 
 val opt_tag_to_opt_bytes: option_nt mac_nt -> result (option bytes)
@@ -124,45 +124,45 @@ let opt_tag_to_opt_bytes mac =
   return (
     match optmac with
     | None -> (None <: option bytes)
-    | Some m -> Some (m.mn_mac_value)
+    | Some m -> Some (m.mac_value)
   )
 
 val opt_bytes_to_opt_tag: option bytes -> result (option_nt mac_nt)
 let opt_bytes_to_opt_tag mac =
   optmac <-- (match mac with
     | None -> (return None)
-    | Some m -> if Seq.length m < 256 then return (Some ({mn_mac_value = m})) else internal_failure "opt_bytes_to_opt_tag: mac too long"
+    | Some m -> if Seq.length m < 256 then return (Some ({mac_value = m})) else internal_failure "opt_bytes_to_opt_tag: mac too long"
   );
   return (option_to_network optmac)
 
 val network_to_message_plaintext: mls_plaintext_nt -> result message_plaintext
 let network_to_message_plaintext pt =
-  sender <-- network_to_sender pt.mpn_sender;
-  content <-- network_to_message_content_pair pt.mpn_content;
+  sender <-- network_to_sender pt.sender;
+  content <-- network_to_message_content_pair pt.content;
   let (|content_type, message_content|) = content in
-  confirmation_tag <-- opt_tag_to_opt_bytes pt.mpn_confirmation_tag;
-  membership_tag <-- opt_tag_to_opt_bytes pt.mpn_membership_tag;
+  confirmation_tag <-- opt_tag_to_opt_bytes pt.confirmation_tag;
+  membership_tag <-- opt_tag_to_opt_bytes pt.membership_tag;
   return ({
-    mp_group_id = pt.mpn_group_id;
-    mp_epoch = Lib.IntTypes.v pt.mpn_epoch;
-    mp_sender = sender;
-    mp_authenticated_data = pt.mpn_authenticated_data;
-    mp_content_type = content_type;
-    mp_message_content = message_content;
-    mp_signature = pt.mpn_signature;
-    mp_confirmation_tag = confirmation_tag;
-    mp_membership_tag = membership_tag;
-  })
+    group_id = pt.group_id;
+    epoch = Lib.IntTypes.v pt.epoch;
+    sender = sender;
+    authenticated_data = pt.authenticated_data;
+    content_type = content_type;
+    message_content = message_content;
+    signature = pt.signature;
+    confirmation_tag = confirmation_tag;
+    membership_tag = membership_tag;
+  } <: message_plaintext)
 
 val network_to_ciphertext_content: #content_type: content_type_nt{valid_network_message_content_type content_type} -> mls_ciphertext_content_nt content_type -> result (message_ciphertext_content (network_to_message_content_type_tot content_type))
 let network_to_ciphertext_content #content_type ciphertext_content =
-  content <-- network_to_message_content ciphertext_content.mccn_content;
-  confirmation_tag <-- opt_tag_to_opt_bytes ciphertext_content.mccn_confirmation_tag;
+  content <-- network_to_message_content ciphertext_content.content;
+  confirmation_tag <-- opt_tag_to_opt_bytes ciphertext_content.confirmation_tag;
   return ({
-    mcc_message_content = content;
-    mcc_signature = ciphertext_content.mccn_signature;
-    mcc_confirmation_tag = confirmation_tag;
-    mcc_padding = ciphertext_content.mccn_signature;
+    message_content = content;
+    signature = ciphertext_content.signature;
+    confirmation_tag = confirmation_tag;
+    padding = ciphertext_content.signature;
   })
 
 val get_ciphertext_sample: ciphersuite -> bytes -> bytes
@@ -174,40 +174,40 @@ let get_ciphertext_sample cs ct =
 
 val decrypt_sender_data: ciphersuite -> message_ciphertext -> bytes -> result mls_sender_data_nt
 let decrypt_sender_data cs ct sender_data_secret =
-  if not (Seq.length ct.mc_group_id < 256) then (
+  if not (Seq.length ct.group_id < 256) then (
     internal_failure "decrypt_sender_data: group_id too long"
-  ) else if not (ct.mc_epoch < pow2 64) then (
+  ) else if not (ct.epoch < pow2 64) then (
     internal_failure "decrypt_sender_data: epoch too big"
   ) else (
-    let ciphertext_sample = get_ciphertext_sample cs ct.mc_ciphertext in
+    let ciphertext_sample = get_ciphertext_sample cs ct.ciphertext in
     sender_data_key <-- expand_with_label cs sender_data_secret (string_to_bytes "key") ciphertext_sample (aead_key_length cs);
     sender_data_nonce <-- expand_with_label cs sender_data_secret (string_to_bytes "nonce") ciphertext_sample (aead_nonce_length cs);
     let ad = ps_mls_sender_data_aad.serialize ({
-      msdan_group_id = ct.mc_group_id;
-      msdan_epoch = u64 ct.mc_epoch;
-      msdan_content_type = message_content_type_to_network ct.mc_content_type;
+      group_id = ct.group_id;
+      epoch = u64 ct.epoch;
+      content_type = message_content_type_to_network ct.content_type;
     }) in
-    sender_data <-- aead_decrypt cs sender_data_key sender_data_nonce ad ct.mc_encrypted_sender_data;
+    sender_data <-- aead_decrypt cs sender_data_key sender_data_nonce ad ct.encrypted_sender_data;
     from_option "decrypt_sender_data: malformed sender data" ((ps_to_pse ps_mls_sender_data).parse_exact sender_data)
   )
 
-val decrypt_ciphertext_content: cs:ciphersuite -> ct:message_ciphertext -> aead_key cs -> aead_nonce cs -> result (mls_ciphertext_content_nt (message_content_type_to_network ct.mc_content_type))
+val decrypt_ciphertext_content: cs:ciphersuite -> ct:message_ciphertext -> aead_key cs -> aead_nonce cs -> result (mls_ciphertext_content_nt (message_content_type_to_network ct.content_type))
 let decrypt_ciphertext_content cs ct key nonce =
-  if not (Seq.length ct.mc_group_id < 256) then (
+  if not (Seq.length ct.group_id < 256) then (
     internal_failure "decrypt_ciphertext_content: group_id too long"
-  ) else if not (ct.mc_epoch < pow2 64) then (
+  ) else if not (ct.epoch < pow2 64) then (
     internal_failure "decrypt_ciphertext_content: epoch too big"
-  ) else if not (Seq.length ct.mc_authenticated_data < pow2 32) then (
+  ) else if not (Seq.length ct.authenticated_data < pow2 32) then (
     internal_failure "decrypt_ciphertext_content: authenticated_data too long"
   ) else (
-    let content_type = message_content_type_to_network ct.mc_content_type in
+    let content_type = message_content_type_to_network ct.content_type in
     let ad = ps_mls_ciphertext_content_aad.serialize ({
-      mccan_group_id = ct.mc_group_id;
-      mccan_epoch = u64 ct.mc_epoch;
-      mccan_content_type = content_type;
-      mccan_authenticated_data = ct.mc_authenticated_data;
+      group_id = ct.group_id;
+      epoch = u64 ct.epoch;
+      content_type = content_type;
+      authenticated_data = ct.authenticated_data;
     }) in
-    ciphertext_content <-- aead_decrypt cs key nonce ad ct.mc_ciphertext;
+    ciphertext_content <-- aead_decrypt cs key nonce ad ct.ciphertext;
     from_option "decrypt_ciphertext_content: malformed ciphertext content" ((ps_to_pse (ps_mls_ciphertext_content content_type)).parse_exact ciphertext_content)
   )
 
@@ -229,44 +229,45 @@ let apply_reuse_guard cs reuse_guard nonce =
 val network_to_encrypted_sender_data: mls_sender_data_nt -> encrypted_sender_data_content
 let network_to_encrypted_sender_data sd =
   ({
-    esdc_sender = Lib.IntTypes.v sd.msdn_sender;
-    esdc_generation = Lib.IntTypes.v sd.msdn_generation;
-    esdc_reuse_guard = sd.msdn_reuse_guard;
+    sender = Lib.IntTypes.v sd.sender;
+    generation = Lib.IntTypes.v sd.generation;
+    reuse_guard = sd.reuse_guard;
   })
 
 val network_to_message_ciphertext: mls_ciphertext_nt -> result message_ciphertext
 let network_to_message_ciphertext ct =
-  content_type <-- network_to_message_content_type ct.mcn_content_type;
+  content_type <-- network_to_message_content_type ct.content_type;
   return ({
-    mc_group_id = ct.mcn_group_id;
-    mc_epoch = Lib.IntTypes.v ct.mcn_epoch;
-    mc_content_type = content_type;
-    mc_authenticated_data = ct.mcn_authenticated_data;
-    mc_encrypted_sender_data = ct.mcn_encrypted_sender_data;
-    mc_ciphertext = ct.mcn_ciphertext;
+    group_id = ct.group_id;
+    epoch = Lib.IntTypes.v ct.epoch;
+    content_type = content_type;
+    authenticated_data = ct.authenticated_data;
+    encrypted_sender_data = ct.encrypted_sender_data;
+    ciphertext = ct.ciphertext;
   })
 
 val message_ciphertext_to_message: #cs:ciphersuite -> (nat -> result (ratchet_output cs)) -> bytes -> message_ciphertext -> result (message & message_auth)
 let message_ciphertext_to_message #cs get_key_nonce sender_data_secret ct =
   sender_data <-- decrypt_sender_data cs ct sender_data_secret;
   let sender_data = network_to_encrypted_sender_data sender_data in
-  rs_output <-- get_key_nonce sender_data.esdc_generation;
-  let nonce = rs_output.ro_nonce in
-  let key = rs_output.ro_key in
-  let patched_nonce = apply_reuse_guard cs sender_data.esdc_reuse_guard nonce in
+  rs_output <-- get_key_nonce sender_data.generation;
+  let nonce = rs_output.nonce in
+  let key = rs_output.key in
+  let patched_nonce = apply_reuse_guard cs sender_data.reuse_guard nonce in
   ciphertext_content_bytes <-- decrypt_ciphertext_content cs ct key patched_nonce;
   ciphertext_content <-- network_to_ciphertext_content ciphertext_content_bytes;
-  return ({
-    m_group_id = ct.mc_group_id;
-    m_epoch = ct.mc_epoch;
-    m_sender = ({
-      s_sender_type = ST_member;
-      s_sender_id = sender_data.esdc_sender;
+  return (({
+    group_id = ct.group_id;
+    epoch = ct.epoch;
+    sender = ({
+      sender_type = ST_member;
+      sender_id = sender_data.sender;
     });
-    m_authenticated_data = ct.mc_authenticated_data;
-    m_content_type = ct.mc_content_type;
-    m_message_content = ciphertext_content.mcc_message_content;
-  }, {
-    m_signature = ciphertext_content.mcc_signature;
-    m_confirmation_tag = ciphertext_content.mcc_confirmation_tag;
-  })
+    authenticated_data = ct.authenticated_data;
+    content_type = ct.content_type;
+    message_content = ciphertext_content.message_content;
+  } <: message), ({
+    signature = ciphertext_content.signature;
+    confirmation_tag = ciphertext_content.confirmation_tag;
+  } <: message_auth))
+
