fstar/new/MLS.TreeKEM.Types.fst
@@ -6,8 +6,8 @@ open Lib.ByteSequence
 open Lib.IntTypes
 
 noeq type member_info (cs:ciphersuite) = {
-  mi_public_key: hpke_public_key cs;
-  mi_version: nat;
+  public_key: hpke_public_key cs;
+  version: nat;
 }
 
 //TODO: move this in Crypto.fsti?
@@ -17,12 +17,12 @@ noeq type path_secret_ciphertext (cs:ciphersuite) = {
 }
 
 noeq type key_package (cs:ciphersuite) = {
-  kp_public_key: hpke_public_key cs;
-  kp_version: nat;
-  kp_last_group_context: bytes; //Related to version, correspond to the additional data used in the ciphertexts
-  kp_unmerged_leafs: list nat;
-  kp_path_secret_from: direction;
-  kp_path_secret_ciphertext: list (path_secret_ciphertext cs);
+  public_key: hpke_public_key cs;
+  version: nat;
+  last_group_context: bytes; //Related to version, correspond to the additional data used in the ciphertexts
+  unmerged_leafs: list nat;
+  path_secret_from: direction;
+  path_secret_ciphertext: list (path_secret_ciphertext cs);
 }
 
 type treekem (cs:ciphersuite) (l:nat) (n:tree_size l) = tree l n (option (member_info cs)) (option (key_package cs))
