fstar/new/MLS.TreeSyncTreeKEMBinder.fst
@@ -6,8 +6,8 @@ open MLS.Parser
 open MLS.NetworkTypes
 open MLS.Tree
 open MLS.NetworkBinder
-module TS = MLS.TreeSync.Types
-module TK = MLS.TreeKEM.Types
+open MLS.TreeSync.Types
+open MLS.TreeKEM.Types
 open MLS.Result
 
 #set-options "--fuel 1 --ifuel 1"
@@ -24,49 +24,49 @@ let secret_to_pub b =
   let open Lib.IntTypes in
   Seq.seq_of_list (List.Tot.map (fun x -> byte (v x)) (Seq.seq_to_list b))
 
-let encrypted_path_secret_nt_to_tk (cs:ciphersuite) (x:hpke_ciphertext_nt): result (TK.path_secret_ciphertext cs) =
-  if not (Seq.length x.hcn_kem_output = hpke_kem_output_length cs) then
+let encrypted_path_secret_nt_to_tk (cs:ciphersuite) (x:hpke_ciphertext_nt): result (path_secret_ciphertext cs) =
+  if not (Seq.length x.kem_output = hpke_kem_output_length cs) then
     internal_failure "encrypted_path_secret_nt_to_tk: kem_output has wrong length"
   else
     return ({
-      TK.kem_output = x.hcn_kem_output;
-      TK.ciphertext = x.hcn_ciphertext;
+      kem_output = x.kem_output;
+      ciphertext = x.ciphertext;
     })
 
-val treesync_to_treekem_node_package: cs:ciphersuite -> nat -> TS.node_package_t -> result (TK.key_package cs)
+val treesync_to_treekem_node_package: cs:ciphersuite -> nat -> node_package_t -> result (key_package cs)
 let treesync_to_treekem_node_package cs nb_left_leaves np =
   content <-- from_option "treesync_to_treekem_node_package: Couldn't parse node content"
-    ((ps_to_pse ps_node_package_content).parse_exact (pub_to_secret np.TS.np_content));
-  path_secret_ciphertext <-- mapM (encrypted_path_secret_nt_to_tk cs) (Seq.seq_to_list content.npc_encrypted_path_secret);
+    ((ps_to_pse ps_node_package_content).parse_exact (pub_to_secret np.content));
+  path_secret_ciphertext <-- mapM (encrypted_path_secret_nt_to_tk cs) (Seq.seq_to_list content.encrypted_path_secret);
   unmerged_leaves <-- mapM (fun (unmerged_leaf:nat) ->
     if not (nb_left_leaves <= unmerged_leaf) then
       error "treesync_to_treekem_node_package: unmerged_leaf index too small"
     else
       return ((unmerged_leaf - nb_left_leaves) <: nat)
-  ) np.TS.np_unmerged_leafs;
-  if not (Seq.length content.npc_public_key = hpke_public_key_length cs) then
+  ) np.unmerged_leafs;
+  if not (Seq.length content.public_key = hpke_public_key_length cs) then
     error "treesync_to_treekem_node_package: public key has wrong length"
   else (
     return ({
-      TK.kp_public_key = content.npc_public_key;
-      TK.kp_version = np.TS.np_version;
-      TK.kp_last_group_context = content.npc_last_group_context;
-      TK.kp_unmerged_leafs = unmerged_leaves;
-      TK.kp_path_secret_from = (np.TS.np_content_dir);
-      TK.kp_path_secret_ciphertext = path_secret_ciphertext;
+      public_key = content.public_key;
+      version = np.version;
+      last_group_context = content.last_group_context;
+      unmerged_leafs = unmerged_leaves;
+      path_secret_from = (np.content_dir);
+      path_secret_ciphertext = path_secret_ciphertext;
     })
   )
 
-val treesync_to_treekem_aux: #l:nat -> #n:tree_size l -> cs:ciphersuite -> nat -> TS.treesync l n -> result (TK.treekem cs l n)
+val treesync_to_treekem_aux: #l:nat -> #n:tree_size l -> cs:ciphersuite -> nat -> treesync l n -> result (treekem cs l n)
 let rec treesync_to_treekem_aux #l #n cs nb_left_leaves t =
   match t with
   | TLeaf (_, None) ->
     return (TLeaf None)
   | TLeaf (_, (Some lp)) ->
     lpc <-- from_option "treesync_to_treekem: Couldn't parse leaf content"
-      ((ps_to_pse ps_leaf_package_content).parse_exact (pub_to_secret lp.TS.lp_content));
-    if Seq.length lpc.lpc_public_key = hpke_public_key_length cs then
-      return (TLeaf (Some ({TK.mi_public_key = lpc.lpc_public_key; TK.mi_version = lp.TS.lp_version})))
+      ((ps_to_pse ps_leaf_package_content).parse_exact (pub_to_secret lp.content));
+    if Seq.length lpc.public_key = hpke_public_key_length cs then
+      return (TLeaf (Some ({public_key = lpc.public_key; version = lp.version} <: member_info cs)))
     else
       error "treesync_to_treekem: public key has wrong length"
   | TSkip _ t' ->
@@ -83,56 +83,56 @@ let rec treesync_to_treekem_aux #l #n cs nb_left_leaves t =
       return (TNode (Some kp) tk_left tk_right)
   end
 
-val treesync_to_treekem: #l:nat -> #n:tree_size l -> cs:ciphersuite -> TS.treesync l n -> result (TK.treekem cs l n)
+val treesync_to_treekem: #l:nat -> #n:tree_size l -> cs:ciphersuite -> treesync l n -> result (treekem cs l n)
 let treesync_to_treekem #l #n cs t =
   treesync_to_treekem_aux cs 0 t
 
-let encrypted_path_secret_tk_to_nt (#cs:ciphersuite) (x:TK.path_secret_ciphertext cs): result (hpke_ciphertext_nt) =
-  if not (Seq.length x.TK.kem_output < pow2 16) then
+let encrypted_path_secret_tk_to_nt (#cs:ciphersuite) (x:path_secret_ciphertext cs): result (hpke_ciphertext_nt) =
+  if not (Seq.length x.kem_output < pow2 16) then
     internal_failure "encrypted_path_secret_tk_to_nt: kem_output too long"
-  else if not (Seq.length x.TK.ciphertext < pow2 16) then
+  else if not (Seq.length x.ciphertext < pow2 16) then
     internal_failure "encrypted_path_secret_tk_to_nt: ciphertext too long"
   else
     return ({
-      hcn_kem_output = x.TK.kem_output;
-      hcn_ciphertext = x.TK.ciphertext;
-    })
+      kem_output = x.kem_output;
+      ciphertext = x.ciphertext;
+    } <: hpke_ciphertext_nt)
 
-val treekem_to_treesync_node_package: #cs:ciphersuite -> nat -> TK.key_package cs -> result TS.external_node_package_t
+val treekem_to_treesync_node_package: #cs:ciphersuite -> nat -> key_package cs -> result external_node_package_t
 let treekem_to_treesync_node_package #cs nb_left_leaves kp =
-  ciphertexts <-- mapM encrypted_path_secret_tk_to_nt kp.TK.kp_path_secret_ciphertext;
+  ciphertexts <-- mapM encrypted_path_secret_tk_to_nt kp.path_secret_ciphertext;
   if not (byte_length ps_hpke_ciphertext ciphertexts < pow2 16) then
     internal_failure "treekem_to_treesync: ciphertexts too long"
-  else if not (Seq.length kp.TK.kp_last_group_context < pow2 64) then
+  else if not (Seq.length kp.last_group_context < pow2 64) then
     internal_failure "treekem_to_treesync: last group context too long (internal error)"
   else begin
     Seq.lemma_list_seq_bij ciphertexts;
     let np_content = ps_node_package_content.serialize ({
-      npc_public_key = kp.TK.kp_public_key;
-      npc_encrypted_path_secret = Seq.seq_of_list ciphertexts;
-      npc_last_group_context = kp.TK.kp_last_group_context;
-    }) in
-    return ({
-      TS.np_version = kp.TK.kp_version;
-      TS.np_content_dir = kp.TK.kp_path_secret_from;
-      TS.np_unmerged_leafs = List.Tot.map (fun (x:nat) -> (x + nb_left_leaves <: nat)) kp.TK.kp_unmerged_leafs;
-      TS.np_parent_hash = Seq.empty;
-      TS.np_content = secret_to_pub np_content;
-    } <: TS.external_node_package_t)
+      public_key = kp.public_key;
+      encrypted_path_secret = Seq.seq_of_list ciphertexts;
+      last_group_context = kp.last_group_context;
+    } <: node_package_content_nt) in
+    return (({
+      version = kp.version;
+      content_dir = kp.path_secret_from;
+      unmerged_leafs = List.Tot.map (fun (x:nat) -> (x + nb_left_leaves <: nat)) kp.unmerged_leafs;
+      parent_hash = Seq.empty;
+      content = secret_to_pub np_content;
+    } <: node_package_t) <: external_node_package_t)
   end
 
-val treekem_to_treesync_aux: #l:nat -> #n:tree_size l -> #i:leaf_index n -> #cs:ciphersuite -> nat -> TS.leaf_package_t -> TK.pathkem cs l n i -> result (TS.external_pathsync l n i)
+val treekem_to_treesync_aux: #l:nat -> #n:tree_size l -> #i:leaf_index n -> #cs:ciphersuite -> nat -> leaf_package_t -> pathkem cs l n i -> result (external_pathsync l n i)
 let rec treekem_to_treesync_aux #l #n #i #cs nb_left_leaves old_leaf_package pk =
   match pk with
   | PLeaf mi ->
     return (PLeaf ({
-      TS.lp_credential = old_leaf_package.TS.lp_credential;
-      TS.lp_version = mi.TK.mi_version;
-      TS.lp_content = secret_to_pub (ps_leaf_package_content.serialize ({
-        lpc_public_key = mi.TK.mi_public_key;
+      credential = old_leaf_package.credential;
+      version = (mi <: member_info cs).version;
+      content = secret_to_pub (ps_leaf_package_content.serialize ({
+        public_key = (mi <: member_info cs).public_key;
       }));
-      TS.lp_extensions = old_leaf_package.TS.lp_extensions; //TODO probably the parent hash should change?
-      TS.lp_signature = old_leaf_package.TS.lp_signature; //TODO the signature definitely has to change
+      extensions = old_leaf_package.extensions; //TODO probably the parent hash should change?
+      signature = old_leaf_package.signature; //TODO the signature definitely has to change
     }))
   | PSkip _ pk' ->
     result <-- treekem_to_treesync_aux nb_left_leaves old_leaf_package pk';
@@ -144,7 +144,7 @@ let rec treekem_to_treesync_aux #l #n #i #cs nb_left_leaves old_leaf_package pk 
     np <-- treekem_to_treesync_node_package nb_left_leaves kp;
     return (PNode np next)
 
-val treekem_to_treesync: #l:nat -> #n:tree_size l -> #i:leaf_index n -> #cs:ciphersuite -> TS.leaf_package_t -> TK.pathkem cs l n i -> result (TS.external_pathsync l n i)
+val treekem_to_treesync: #l:nat -> #n:tree_size l -> #i:leaf_index n -> #cs:ciphersuite -> leaf_package_t -> pathkem cs l n i -> result (external_pathsync l n i)
 let treekem_to_treesync #l #n #i #cs old_leaf_package pk =
   treekem_to_treesync_aux 0 old_leaf_package pk
 
