fstar/new/MLS.Test.CommitTranscript.fst
@@ -16,7 +16,7 @@ open MLS.Result
 
 val test_commit_transcript_one: commit_transcript_test -> ML bool
 let test_commit_transcript_one t =
-  match uint16_to_ciphersuite t.ctt_cipher_suite with
+  match uint16_to_ciphersuite t.cipher_suite with
   | ProtocolError s -> begin
     IO.print_string ("Skipping one test because of missing ciphersuite: '" ^ s ^ "'\n");
     true
@@ -26,18 +26,18 @@ let test_commit_transcript_one t =
     false
   end
   | Success cs -> begin
-    let ciphersuite_network = extract_option "malformed credential" ((ps_to_pse ps_credential).parse_exact (hex_string_to_bytes t.ctt_credential)) in
-    let commit_network = extract_option "malformed MLSPlaintext(Commit)" ((ps_to_pse ps_mls_plaintext).parse_exact (hex_string_to_bytes t.ctt_commit)) in
+    let ciphersuite_network = extract_option "malformed credential" ((ps_to_pse ps_credential).parse_exact (hex_string_to_bytes t.credential)) in
+    let commit_network = extract_option "malformed MLSPlaintext(Commit)" ((ps_to_pse ps_mls_plaintext).parse_exact (hex_string_to_bytes t.commit)) in
     let commit_plaintext = extract_result (network_to_message_plaintext commit_network) in
     let (commit_message, commit_auth) = message_plaintext_to_message commit_plaintext in
-    let computed_confirmed_transcript_hash = extract_result (compute_confirmed_transcript_hash cs commit_message commit_auth.m_signature (hex_string_to_bytes t.ctt_interim_transcript_hash_before)) in
+    let computed_confirmed_transcript_hash = extract_result (compute_confirmed_transcript_hash cs commit_message commit_auth.signature (hex_string_to_bytes t.interim_transcript_hash_before)) in
     let computed_interim_transcript_hash = extract_result (compute_interim_transcript_hash cs commit_auth computed_confirmed_transcript_hash) in
-    let computed_confirmation_tag = extract_result (compute_message_confirmation_tag cs (hex_string_to_bytes t.ctt_confirmation_key) computed_confirmed_transcript_hash) in
-    let computed_membership_tag = extract_result (compute_message_membership_tag cs (hex_string_to_bytes t.ctt_membership_key) commit_message commit_auth (hex_string_to_bytes t.ctt_group_context)) in
-    let confirmed_transcript_hash_ok = check_equal "confirmed_transcript_hash" string_to_string (t.ctt_confirmed_transcript_hash_after) (bytes_to_hex_string computed_confirmed_transcript_hash) in
-    let interim_transcript_hash_ok = check_equal "interim_transcript_hash" string_to_string (t.ctt_interim_transcript_hash_after) (bytes_to_hex_string computed_interim_transcript_hash) in
+    let computed_confirmation_tag = extract_result (compute_message_confirmation_tag cs (hex_string_to_bytes t.confirmation_key) computed_confirmed_transcript_hash) in
+    let computed_membership_tag = extract_result (compute_message_membership_tag cs (hex_string_to_bytes t.membership_key) commit_message commit_auth (hex_string_to_bytes t.group_context)) in
+    let confirmed_transcript_hash_ok = check_equal "confirmed_transcript_hash" string_to_string (t.confirmed_transcript_hash_after) (bytes_to_hex_string computed_confirmed_transcript_hash) in
+    let interim_transcript_hash_ok = check_equal "interim_transcript_hash" string_to_string (t.interim_transcript_hash_after) (bytes_to_hex_string computed_interim_transcript_hash) in
     let confirmation_tag_ok =
-      match commit_auth.m_confirmation_tag with
+      match commit_auth.confirmation_tag with
       | Some expected_confirmation_tag ->
         check_equal "confirmation_tag" string_to_string (bytes_to_hex_string expected_confirmation_tag) (bytes_to_hex_string computed_confirmation_tag)
       | _ ->
@@ -45,23 +45,23 @@ let test_commit_transcript_one t =
         false
     in
     let membership_tag_ok =
-      match commit_network.mpn_membership_tag with
+      match commit_network.membership_tag with
       | Some_nt expected_membership_tag ->
-        check_equal "membership_tag" string_to_string (bytes_to_hex_string expected_membership_tag.mn_mac_value) (bytes_to_hex_string computed_membership_tag)
+        check_equal "membership_tag" string_to_string (bytes_to_hex_string expected_membership_tag.mac_value) (bytes_to_hex_string computed_membership_tag)
       | _ ->
         IO.print_string "Missing membership tag\n";
         false
     in
     let signature_ok =
-      if not (let cs_int = Lib.IntTypes.v t.ctt_cipher_suite in cs_int = 1 || cs_int = 3) then (
+      if not (let cs_int = Lib.IntTypes.v t.cipher_suite in cs_int = 1 || cs_int = 3) then (
         IO.print_string "Skipping signature check because only Ed25519 is supported\n";
         true
       ) else (
         match ciphersuite_network with
         | C_basic cred ->
-          if not (Seq.length cred.bcn_signature_key = sign_public_key_length cs) then false
-          else if not (Seq.length commit_auth.m_signature = sign_signature_length cs) then false
-          else extract_result (check_message_signature cs cred.bcn_signature_key commit_auth.m_signature commit_message (hex_string_to_bytes t.ctt_group_context))
+          if not (Seq.length cred.signature_key = sign_public_key_length cs) then false
+          else if not (Seq.length commit_auth.signature = sign_signature_length cs) then false
+          else extract_result (check_message_signature cs cred.signature_key commit_auth.signature commit_message (hex_string_to_bytes t.group_context))
         | _ -> false
       )
     in
