fstar/new/MLS.Test.Encryption.fst
@@ -18,16 +18,16 @@ val test_leaf_generation: #cs:ciphersuite -> bytes -> ratchet_state cs -> encryp
 let test_leaf_generation #cs sender_data_secret r_state test =
   let r_output = extract_result (ratchet_get_key r_state) in
   let r_next_state = extract_result (ratchet_next_state r_state) in
-  let key_ok = check_equal "key" string_to_string test.elgt_key (bytes_to_hex_string r_output.ro_key) in
-  let nonce_ok = check_equal "nonce" string_to_string test.elgt_nonce (bytes_to_hex_string r_output.ro_nonce) in
-  let message_plaintext_network = extract_option "bad plaintext" ((ps_to_pse ps_mls_plaintext).parse_exact (hex_string_to_bytes test.elgt_plaintext)) in
-  let message_ciphertext_network = extract_option "bad ciphertext" ((ps_to_pse ps_mls_ciphertext).parse_exact (hex_string_to_bytes test.elgt_ciphertext)) in
+  let key_ok = check_equal "key" string_to_string test.key (bytes_to_hex_string r_output.key) in
+  let nonce_ok = check_equal "nonce" string_to_string test.nonce (bytes_to_hex_string r_output.nonce) in
+  let message_plaintext_network = extract_option "bad plaintext" ((ps_to_pse ps_mls_plaintext).parse_exact (hex_string_to_bytes test.plaintext)) in
+  let message_ciphertext_network = extract_option "bad ciphertext" ((ps_to_pse ps_mls_ciphertext).parse_exact (hex_string_to_bytes test.ciphertext)) in
   let message_plaintext = extract_result (network_to_message_plaintext message_plaintext_network) in
   let message_ciphertext = extract_result (network_to_message_ciphertext message_ciphertext_network) in
   let message_1 = message_plaintext_to_message message_plaintext in
-  let message_2 = extract_result (message_ciphertext_to_message (fun i -> if r_state.rs_generation <= i then ratchet_get_generation_key r_state i else internal_failure "ratchet: generation not available") sender_data_secret message_ciphertext) in
+  let message_2 = extract_result (message_ciphertext_to_message (fun i -> if r_state.generation <= i then ratchet_get_generation_key r_state i else internal_failure "ratchet: generation not available") sender_data_secret message_ciphertext) in
   let plaintext_eq_ciphertext_ok = test_equality message_1 message_2 in
-  let sender_ok = (fst message_1).m_sender.s_sender_type = MLS.TreeDEM.Message.Framing.ST_member && (let open FStar.Mul in 2*(fst message_1).m_sender.s_sender_id = r_state.rs_node) in
+  let sender_ok = (fst message_1).sender.sender_type = MLS.TreeDEM.Message.Framing.ST_member && (let open FStar.Mul in 2*(fst message_1).sender.sender_id = r_state.node) in
   (key_ok && nonce_ok && plaintext_eq_ciphertext_ok && sender_ok, r_next_state)
 
 val test_leaf_generations: #cs:ciphersuite -> bytes -> ratchet_state cs -> list encryption_leaf_generation_test -> ML bool
@@ -64,11 +64,11 @@ let test_leaves cs l n encryption_secret sender_data_secret leaf_tests =
 
 val test_encryption_one: encryption_test -> ML bool
 let test_encryption_one t =
-  if FStar.UInt16.v t.et_cipher_suite <> 3 then (
+  if FStar.UInt16.v t.cipher_suite <> 3 then (
     IO.print_string "Skipping test because only Chacha20Poly1305 is supported\n";
     true
   ) else (
-    match uint16_to_ciphersuite t.et_cipher_suite with
+    match uint16_to_ciphersuite t.cipher_suite with
     | ProtocolError s -> begin
       IO.print_string ("Skipping one test because of missing ciphersuite: '" ^ s ^ "'\n");
       true
@@ -78,12 +78,12 @@ let test_encryption_one t =
       false
     end
     | Success cs -> begin
-      let n_leaves = UInt32.v t.et_n_leaves in
+      let n_leaves = UInt32.v t.n_leaves in
       let n_nodes = n_leaves + n_leaves - 1 in
       let l = if n_nodes > 0 then (MLS.TreeMath.Internal.log2 n_nodes) + 1 else failwith "there cannot be 0 leaves!" in
       let leaves_ok =
-        if List.Tot.length t.et_leaves <= n_leaves then
-          test_leaves cs l n_leaves (hex_string_to_bytes t.et_encryption_secret) (hex_string_to_bytes t.et_sender_data_secret) t.et_leaves
+        if List.Tot.length t.leaves <= n_leaves then
+          test_leaves cs l n_leaves (hex_string_to_bytes t.encryption_secret) (hex_string_to_bytes t.sender_data_secret) t.leaves
         else
           failwith "list leaves is too big!"
       in
