fstar/new/MLS.TreeSync.ExternalPath.fst
@@ -3,12 +3,12 @@ module MLS.TreeSync.ExternalPath
 open Lib.ByteSequence
 open MLS.Tree
 open MLS.Crypto
-open MLS.TreeSync.Types
+open MLS.NetworkTypes
+open MLS.NetworkBinder
 open MLS.TreeSync.ParentHash
 open MLS.TreeSync.IntegrityCheck
 open MLS.TreeSync.Extensions
-open MLS.NetworkTypes
-open MLS.NetworkBinder
+open MLS.TreeSync.Types
 open MLS.Parser
 open MLS.Result
 
@@ -26,22 +26,22 @@ let rec external_pathsync_to_pathsync_aux #l #n #i cs opt_sign_key parent_parent
         if not (Seq.length parent_parent_hash < 256) then
           internal_failure "external_pathsync_to_pathsync_aux: parent hash too long"
         else (
-          new_extensions <-- set_parent_hash_extension lp.lp_extensions ({phen_parent_hash = parent_parent_hash});
-          let lp = ({lp with lp_extensions = new_extensions}) in
+          new_extensions <-- set_parent_hash_extension lp.extensions ({parent_hash = parent_parent_hash});
+          let lp = ({lp with extensions = new_extensions}) in
           key_package <-- treesync_to_keypackage cs lp;
           let leaf_package_bytes = ps_key_package_tbs.serialize (key_package_get_tbs key_package) in
           new_signature <-- sign_sign cs sign_key leaf_package_bytes entropy;
-          return ({lp with lp_signature = new_signature})
+          return ({lp with signature = new_signature} <: leaf_package_t)
         )
       )
     );
-    let parent_hash_ext = get_parent_hash_extension lp.lp_extensions in
+    let parent_hash_ext = get_parent_hash_extension lp.extensions in
     //TODO: hack while openmls' test vectors are broken
     if not (IE_Good? leaf_errors || (match leaf_errors with |IE_Errors [IE_LeafError LIE_ExtensionsNotInCapabilities _] -> true | _ -> false)) then
       error "external_pathsync_to_pathsync_aux: invalid leaf"
     else if not (Some? parent_hash_ext) then
       error "external_pathsync_to_pathsync_aux: leaf don't contain any parent hash"
-    else if not ((Some?.v parent_hash_ext).phen_parent_hash = parent_parent_hash) then
+    else if not ((Some?.v parent_hash_ext).parent_hash = parent_parent_hash) then
       error "external_pathsync_to_pathsync_aux: leaf contain an invalid parent hash"
     else
       return (PLeaf (Some lp))
@@ -52,9 +52,9 @@ let rec external_pathsync_to_pathsync_aux #l #n #i cs opt_sign_key parent_parent
     let (|dir, next_i|) = child_index l i in
     let (child, sibling) = order_subtrees dir (left, right) in
     let child_nb_left_leaves = if dir = Left then nb_left_leaves else nb_left_leaves + (pow2 (l-1)) in
-    parent_hash <-- compute_parent_hash_from_dir cs np.np_content parent_parent_hash nb_left_leaves t dir;
+    parent_hash <-- compute_parent_hash_from_dir cs np.content parent_parent_hash nb_left_leaves t dir;
     result_p_next <-- external_pathsync_to_pathsync_aux cs opt_sign_key parent_hash child_nb_left_leaves child p_next;
-    return (PNode (Some ({np with np_parent_hash = parent_parent_hash;})) result_p_next)
+    return (PNode (Some ({np with parent_hash = parent_parent_hash;})) result_p_next)
 
 val external_pathsync_to_pathsync: #l:nat -> #n:tree_size l -> #i:leaf_index n -> cs:ciphersuite -> option (sign_private_key cs & randomness (sign_nonce_length cs)) -> treesync l n -> external_pathsync l n i -> result (pathsync l n i)
 let external_pathsync_to_pathsync #l #n #i cs opt_sign_key t p =
