fstar/new/MLS.TreeSync.Hash.fst
@@ -14,8 +14,8 @@ open MLS.NetworkBinder
 #set-options "--fuel 1 --ifuel 1 --z3rlimit 50"
 
 noeq type leaf_node_tree_hash_input_nt = {
-  lnthi_node_index: uint32;
-  lnthi_key_package: option_nt key_package_nt;
+  node_index: uint32;
+  key_package: option_nt key_package_nt;
 }
 
 val ps_leaf_node_tree_hash_input: parser_serializer leaf_node_tree_hash_input_nt
@@ -27,16 +27,16 @@ let ps_leaf_node_tree_hash_input =
       ps_option (ps_key_package)
     )
   (fun (|node_index, key_package|) -> {
-    lnthi_node_index = node_index;
-    lnthi_key_package = key_package;
+    node_index = node_index;
+    key_package = key_package;
   })
-  (fun x -> (|x.lnthi_node_index, x.lnthi_key_package|))
+  (fun x -> (|x.node_index, x.key_package|))
 
 noeq type parent_node_tree_hash_input_nt = {
-  pnthi_node_index: uint32;
-  pnthi_parent_node: option_nt parent_node_nt;
-  pnthi_left_hash: blbytes ({min=0;max=255});
-  pnthi_right_hash: blbytes ({min=0;max=255});
+  node_index: uint32;
+  parent_node: option_nt parent_node_nt;
+  left_hash: blbytes ({min=0;max=255});
+  right_hash: blbytes ({min=0;max=255});
 }
 
 #push-options "--ifuel 2"
@@ -51,12 +51,12 @@ let ps_parent_node_tree_hash_input =
       ps_bytes _
     )
   (fun (|node_index, (|parent_node, (|left_hash, right_hash|)|)|) -> {
-    pnthi_node_index = node_index;
-    pnthi_parent_node = parent_node;
-    pnthi_left_hash = left_hash;
-    pnthi_right_hash = right_hash;
+    node_index = node_index;
+    parent_node = parent_node;
+    left_hash = left_hash;
+    right_hash = right_hash;
   })
-  (fun x -> (|x.pnthi_node_index, (|x.pnthi_parent_node, (|x.pnthi_left_hash, x.pnthi_right_hash|)|)|))
+  (fun x -> (|x.node_index, (|x.parent_node, (|x.left_hash, x.right_hash|)|)|))
 #pop-options
 
 val tree_hash: #l:nat -> #n:tree_size l -> cs:ciphersuite -> TM.node_index l -> treesync l n -> result (lbytes (hash_length cs))
@@ -75,8 +75,8 @@ let rec tree_hash #l #n cs ind t =
       internal_failure "tree_hash: node_index too big"
     else
       hash_hash cs (ps_leaf_node_tree_hash_input.serialize ({
-        lnthi_node_index = u32 ind;
-        lnthi_key_package = key_package;
+        node_index = u32 ind;
+        key_package = key_package;
       }))
   | TNode (_, onp) left right ->
     parent_node <-- (
@@ -92,8 +92,8 @@ let rec tree_hash #l #n cs ind t =
       internal_failure "tree_hash: node_index too big"
     else
       hash_hash cs (ps_parent_node_tree_hash_input.serialize ({
-        pnthi_node_index = u32 ind;
-        pnthi_parent_node = parent_node;
-        pnthi_left_hash = left_hash;
-        pnthi_right_hash = right_hash;
+        node_index = u32 ind;
+        parent_node = parent_node;
+        left_hash = left_hash;
+        right_hash = right_hash;
       }))
